\input{header.tex}

\setcounter{theorem}{49}
\begin{exercise}[BH.2.50] 
\begin{solution}
	\begin{enumerate}
		\item First use the LOTP where you condition on the outcome of the first match,
		\begin{align*}
			P(W)& = P(W|W_{1})p + P(W|W_{1}^{C})(1-p).\\
		\end{align*}
		Now use extra conditioning on the outcome of the second match
		\begin{align*}
			P(W|W_{1})& = P(W|W_{1},W_{2})P(W_{2}|W_{1}) + P(W|W_{1},W_{2}^C)P(W_{2}^C|W_{1})\\
			&=1\cdot p + P(W)(1-p).
		\end{align*}
		Similarly, we find that
		\begin{align*}
			P(W|W_{1}^{C}) &= P(W|W_{1}^{C},W_{2})P(W_{2}|W_{1}^{C})+P(W|W_{1}^{C},W_{2}^C)P(W_{2}^C|W_{1}^{C})\\
			&=P(W)p.
		\end{align*}
		Substituting the last two results into the first equation, we have
		\begin{align*}
			P(W) = p^2 + P(W)(1-p)p + P(W)p(1-p) = p^2 +2p(1-p)P(W).
		\end{align*}
		Solving for $P(W)$ gives
		\begin{align*}
			P(W) =\frac{p^2}{1-2p(1-p)}.
		\end{align*}
		\item Skip.
	\end{enumerate}
\end{solution}
\end{exercise}
\input{trailer.tex}
